src/3d/prelude/Actions.fsti
@@ -134,6 +134,23 @@ val validate_with_success_action
       (a:action p1 inv2 l2 b bool)
   : validate_with_action_t p1 (conj_inv inv1 inv2) (l1 `eloc_union` l2) false
 
+val error_handler : Type0
+
+inline_for_extraction noextract
+val validate_with_error_handler (typename: string)
+                                (fieldname: string)
+                                (#nz: _)
+                                (#wk: _)
+                                (#k1:parser_kind nz wk)
+                                (#t1: _)
+                                (#p1:parser k1 t1)
+                                (#inv1:_)
+                                (#l1:eloc)
+                                (#ar:_)
+                                (v1:validate_with_action_t p1 inv1 l1 ar)
+                                (err:error_handler)
+  : validate_with_action_t p1 inv1 l1 ar
+
 inline_for_extraction noextract
 val validate_with_error_action
       (name: string)
